\documentclass[10pt]{article}

\usepackage{amssymb,amsmath,amsthm}
\usepackage{bm}
\usepackage{graphicx,subcaption}
\usepackage[letterpaper, top=1in, left=1in, right=1in, bottom=1in]{geometry}

\newtheorem{definition}{Definition}
\newtheorem{proposition}{Proposition}
\newtheorem{theorem}{Theorem}
\newtheorem{lemma}{Lemma}
\newtheorem{remark}{Remark}

\title{\vspace{-4ex}\textbf{Analytical Uncertainty Propagation with Global Angular Velocity\vspace{-4ex}}}
\date{}

\newcommand{\norm}[1]{\ensuremath{\left\| #1 \right\|}}
\newcommand{\fnorm}[1]{\ensuremath{\left\| #1 \right\|_\mathrm{F}}}
\newcommand{\tr}[1]{\ensuremath{\mathrm{tr}\left( #1 \right)}}
\newcommand{\etr}[1]{\ensuremath{\mathrm{etr}\left\{ #1 \right\}}}
\newcommand{\expect}[1]{\ensuremath{\mathrm{E}\left[ #1 \right]}}
\newcommand{\SO}{\ensuremath{\mathrm{SO(3)}}}
\newcommand{\real}[1]{\ensuremath{\mathbb{R}^{ #1 }}}
\newcommand{\diff}[1]{\ensuremath{\mathrm{d} #1}}

\begin{document}

\maketitle

Consider the following discrete kinematics model where the angular velocity is measured in the inertial reference frame.
\begin{align}
	R_{k+1} &= \exp\left( h(\hat{\Omega}_k+\hat{x}_k) + (H_u\Delta W_u)^\wedge \right)R_k, \label{eqn:attKine} \\
	x_{k+1} &= x_k.
\end{align}

Suppose $(R_k,x_k) \sim \mathcal{MG}(\mu_k,\Sigma_k,P_k,U_k,S_k,V_k)$, we want to find the distribution for $(R_{k+1},x_{k+1})$.
First, we separate the deterministic part and random part.
By the BCH formula, \eqref{eqn:attKine} can be written as
\begin{equation}
	R_{k+1} = \exp\left( h(\hat{\Omega}_k + \mu_k )\right) \exp\left( h(\hat{x}_k-\mu_k) + (H_u\Delta W_u)^\wedge + o(h)\right) R_k.
\end{equation}

The $o(h)$ terms will become $O(h^2)$ after expanding the exponential map and taking the expectation, so the following equation will be considered.
\begin{equation}
	R_{k+1} = \exp\left( h(\hat{\Omega}_k + \hat{\mu}_k )\right) \exp\left( h(\hat{x}_k-\hat{\mu}_k) + (H_u\Delta W_u)^\wedge\right) R_k.
\end{equation}

\section{Original Definition using $Q$}

In this definition, $\nu_R = (QS-SQ^T)^\vee$.

\subsection{Calculating $\expect{R_{k+1}}$}

Let $\delta R_k = \exp\left(h(\hat{\Omega}_k+\hat{\mu}_k)\right)$, then
\begin{align*}
	\expect{R_{k+1}} &= \delta R_k \sum_{i=1}^{\infty} \frac{1}{i!} \expect{\left(h(\hat{x}_k-\hat{\mu}_k)+(H_u\Delta W_u)^\wedge\right)^i R_k} \\
	&= \delta R_k \left( \expect{R_k} + h\expect{(\hat{x}_k-\hat{\mu}_k)R_k} + \frac{1}{2}\expect{((H_u\Delta W_u)^\wedge)^2R_k} \right) \\
	&= \delta R_k \left( \expect{R_k} + h\expect{\widehat{P_k\nu_{R_k}}U_kQ_k}V_k^T + \frac{h}{2}(G_u-\tr{G_u}I)\expect{R_k} \right)
\end{align*}

\subsection{Calculating $\expect{x_{k+1}\nu_{R_{k+1}}^T}$}

Let $\Lambda(A) = (U_{k+1}^TAV_{k+1}S_{k+1}-S_{k+1}V_{k+1}^TA^TU_{k+1})^\vee$, then
\begin{align*}
	\expect{x_{k+1}\nu_{R_{k+1}}^T} &= \sum_{i=1}^\infty \frac{1}{i!} \expect{x_{k+1}\Lambda\left( \delta R_k (h(\hat{x}_k-\hat{\mu}_k)+(H_u\Delta W_u)^\wedge)^i R_k \right)^T} \\
	&= \expect{x_k\Lambda(\delta R_k R_k)^T} + h\expect{x_k\Lambda(\delta R_k(\hat{x}_k-\hat{\mu}_k)R_k)^T} + \frac{1}{2}\expect{x_k\Lambda\left( \delta R_k ((H_u\Delta W_u)^\wedge)^2 R_k \right)^T}
\end{align*}

\noindent Let $\tilde{U} = U_{k+1}^T\delta R_kU_k$, $\tilde{V} = V_{k+1}^TV_k$, $\tilde{S} = \tilde{U}^TS_{k+1}\tilde{V}$, and $\tilde{\nu}_R = (Q_k\tilde{S}^T-\tilde{S}Q_k^T)^\vee$.
Then
\begin{align*}
	\Lambda(\delta R_kR_k) &= (U_{k+1}^T\delta R_kU_kQ_kV_k^TV_{k+1}S_{k+1} - S_{k+1}V_{k+1}^TV_kQ_k^TU_k^T\delta R_k^TU_{k+1})^\vee \\
	&= (\tilde{U}Q_k\tilde{V}^TS_{k+1} - S_{k+1}\tilde{V}Q_k\tilde{U}^T)^\vee \\
	&= \tilde{U}(Q_k\tilde{V}^TS_{k+1}\tilde{U} - \tilde{U}^TS_{k+1}\tilde{V}Q_k)^\vee \\
	&= \tilde{U}(Q_k\tilde{S}^T-\tilde{S}Q^T)^\vee \\
	&= \tilde{U}\tilde{\nu}_R.
\end{align*}

\noindent Also, let $\Gamma_Q = \tr{Q_k\tilde{S}^T}I-Q_k\tilde{S}^T$.
Then
\begin{align*}
	\Lambda(\delta R_k(\hat{x}_k-\hat{\mu}_k)R_k) &= (U_{k+1}^T\delta R_k(\hat{x}_k-\hat{\mu}_k)U_kQ_k\tilde{V}^TS_{k+1} - S_{k+1}\tilde{V}Q_k^TU_k^T(\hat{x}_k-\hat{\mu}_k)^T\delta R_k^TU_{k+1})^\vee \\
	&= (\tilde{U}(U_k^T(x_k-\mu_k))^\wedge Q_k\tilde{V}^TS_{k+1} - S_{k+1}\tilde{V}Q_k^T((U_k^T(x_k-\mu_k))^\wedge)^T\tilde{U}^T)^\vee \\
	&= \tilde{U}((U_k^T(x_k-\mu_k))^\wedge Q_k\tilde{S}^T - \tilde{S}Q_k^T((U_k^T(x_k-\mu_k))^\wedge)^T)^\vee \\
	&= \tilde{U} \left(\tr{Q_k\tilde{S}^T}I - Q_k\tilde{S}^T\right)U_k^T(x_k-\mu_k) \\
	&= \tilde{U}\Gamma_Q U_k^T(x_k-\mu_k).
\end{align*}

\noindent Therefore, the first term on the right hand side is
\begin{align*}
	\expect{x_k\Lambda(\delta R_kR_k)^T} = \mu_k\expect{\tilde{\nu}^T}\tilde{U}^T + P_k\expect{\nu_{R_k}\tilde{\nu}^T}\tilde{U}^T.
\end{align*}

\noindent The second term on the right hand side is
\begin{align*}
	\expect{x_k\Lambda(\delta R_k(\hat{x}_k-\hat{\mu}_k)R_k)^T} &= \expect{x_k(x_k-\mu_k)^TU_k\Gamma_Q^T}\tilde{U}^T \\
	&= \expect{(\Sigma_{c_k} + \mu_k\nu_{R_k}^TP_k^T + P_k\nu_{R_k}\nu_{R_k}^TP_k^T)U_k\Gamma_Q^T} \tilde{U}^T \\
	&= \Sigma_{c_k}U_k\expect{\Gamma_Q}^T\tilde{U}^T + \mu_k\expect{\nu_{R_k}^TP_k^TU_k\Gamma_Q^T}\tilde{U}^T + P_k\expect{\nu_{R_k}\nu_{R_k}^TP_k^TU_k\Gamma_Q^T}\tilde{U}^T.
\end{align*}

\noindent Let $\tilde{\tilde{U}} = U_{k+1}^T\delta R_kG_uU_k$, $\tilde{\tilde{S}} = \tilde{\tilde{U}}^TS_{k+1}\tilde{V}$, and $\tilde{\tilde{\nu}} = (Q_k\tilde{\tilde{S}}^T-\tilde{\tilde{S}}Q_k^T)^\vee$.
Then the third term on the right hand side is
\begin{align*}
	\expect{x_k\Lambda\left( \delta R_k((H_u\Delta W_u)^\wedge)^2 R_k \right)^T} &= h\expect{x_k\Lambda\left( \delta R_k(G_u-\tr{G_u}I)R_k \right)^T} \\
	&= h\expect{x_k\Lambda(\delta R_kG_uR_k)^T} - \tr{G_u}h\expect{x_k\Lambda(\delta R_kR_k)^T} \\
	&= h\left( \mu_k\expect{\tilde{\tilde{\nu}}}^T + P_k\expect{\nu_{R_k}\tilde{\tilde{\nu}}^T} \right)\tilde{\tilde{U}}^T - \tr{G_u}h\left( \mu_k\expect{\tilde{\nu}}^T + P_k\expect{\nu_{R_k}\tilde{\nu}^T} \right)\tilde{U}^T.
\end{align*}

\subsection{Calculating $\expect{\nu_{R_{k+1}}\nu_{R_{k+1}}^T}$}

\begin{align*}
	\expect{\nu_{R_{k+1}}\nu_{R_{k+1}}^T} &= \expect{\sum_{i=1}^\infty \Lambda\left( \delta R_k \frac{(h(\hat{x}_k-\hat{\mu}_k)+(H_u\Delta W_u)^\wedge)^i}{i!} R_k \right) \cdot \sum_{i=1}^\infty \Lambda\left( \delta R_k \frac{(h(\hat{x}_k-\hat{\mu}_k)+(H_u\Delta W_u)^\wedge)^i}{i!} R_k \right)^T } \\
	&= \expect{\Lambda(\delta R_kR_k)\Lambda(\delta R_kR_k)^T} + h\expect{\Lambda(\delta R_kR_k)\Lambda(\delta R_k(\hat{x}_k-\hat{\mu}_k) R_k)^T} \\
	&\qquad + h\expect{\Lambda(\delta R_k(\hat{x}_k-\hat{\mu}_k) R_k)\Lambda(\delta R_kR_k)^T} + \frac{1}{2}\expect{\Lambda(\delta R_kR_k)\Lambda(\delta R_k((H_u\Delta W_u)^\wedge)^2R_k)^T} \\
	&\qquad + \frac{1}{2}\expect{\Lambda(\delta R_k((H_u\Delta W_u)^\wedge)^2R_k)\Lambda(\delta R_kR_k)^T} + \expect{\Lambda(\delta R_k(H_u\Delta W_u)^\wedge R_k)\Lambda(\delta R_k(H_u\Delta W_u)^\wedge R_k)^T}.
\end{align*}

\noindent The first term on the right hand side is
\begin{align*}
	\expect{\Lambda(\delta R_kR_k)\Lambda(\delta R_kR_k)^T} = \tilde{U}\expect{\tilde{\nu}\tilde{\nu}^T}\tilde{U}^T.
\end{align*}

\noindent The second, third term on the right hand side is
\begin{align*}
	\expect{\Lambda(\delta R_kR_k)\Lambda(\delta R_k(\hat{x}_k-\hat{\mu}_k)R_k)^T} &= \tilde{U}\expect{\tilde{\nu}(x_k-\mu_k)^TU_k\Gamma_Q^T}\tilde{U}^T \\
	&= \tilde{U}\expect{\tilde{\nu}\nu_{R_k}^TP_k^TU_k\Gamma_Q^T}\tilde{U}^T.
\end{align*}

\noindent The fourth, fifth term on the right hand side is
\begin{align*}
	\expect{\Lambda(\delta R_kR_k)\Lambda(\delta R_k((H_u\Delta W_u)^\wedge)^2R_k)^T} &= h\expect{\Lambda(\delta R_kR_k) \Lambda(\delta R_k(G_u-\tr{G_u}I)R_k)^T} \\
	&= h\tilde{U}\expect{\tilde{\nu}\tilde{\tilde{\nu}}^T}\tilde{\tilde{U}}^T + \tr{G_u}h\tilde{U}\expect{\tilde{\nu}\tilde{\nu}^T}\tilde{U}^T.
\end{align*}

\noindent The sixth term on the right hand side is
\begin{align*}
	\expect{\Lambda(\delta R_k(H_u\Delta W_u)^\wedge R_k)\Lambda(\delta R_k(H_u\Delta W_u)^\wedge R_k)^T} &= \tilde{U}\expect{\Gamma_QU_k^T(H_u\Delta W_u)^\wedge((H_u\Delta W_u)^\wedge)^TU_k\Gamma_Q^T}\tilde{U}^T \\
	&= \tilde{U}\expect{\Gamma_QU_k^TG_uU_k\Gamma_Q^T}\tilde{U}^T.
\end{align*}

\section{New Definition using $Q^T$}

In this definition, $\nu_R = (SQ-Q^TS)^\vee$

\subsection{Calculating $\expect{R_{k+1}}$}

The calculation for $\expect{R_{k+1}}$ is the same as the original definition.

\subsection{Calculating $\expect{x_{k+1}\nu_{R_{k+1}}^T}$}

Let $\Lambda(A) = (S_{k+1}U_{k+1}^TAV_{k+1} - V_{k+1}^TA^TU_{k+1}S_{k+1})^\vee$, then
\begin{align*}
	\expect{x_{k+1}\nu_{R_{k+1}}^T} &= \sum_{i=1}^\infty \frac{1}{i!} \expect{x_k\Lambda\left( \delta R_k (h(\hat{x}_k-\hat{\mu}_k) + (H_u\Delta W_u)^\wedge)^i R_k \right)^T} \\
	&= \expect{x_k\Lambda(\delta R_kR_k)^T} + h\expect{x_k\Lambda(\delta R_k(\hat{x}_k-\hat{\mu}_k)R_k)} + \frac{1}{2}\expect{x_k\Lambda\left( \delta R_k((H_u\Delta W_u)^\wedge)^2 R_k \right)}.
\end{align*}

\noindent Let $\tilde{\nu} = (\tilde{S}^TQ_k-Q_k^T\tilde{S})^\vee$, then
\begin{align*}
	\Lambda(\delta R_kR_k) &= (S_{k+1}U_{k+1}^T\delta R_kU_kQ_kV_k^TV_{k+1} - V_{k+1}^TV_kQ_k^TU_k^T\delta R_k^TU_{k+1}S_{k+1})^\vee \\
	&= (S_{k+1}\tilde{U}Q_k\tilde{V}^T - \tilde{V}Q_k^T\tilde{U}^TS_{k+1})^\vee \\
	&= \tilde{V}(\tilde{V}^TS_{k+1}\tilde{U}Q_k - Q_k^T\tilde{U}^TS_{k+1}\tilde{V})^\vee \\
	&= \tilde{V}(\tilde{S}^TQ_k - Q_k^T\tilde{S})^\vee \\
	&= \tilde{V}\tilde{\nu}.
\end{align*}

\noindent Let $\Gamma_Q = \left(\tr{Q_k^T\tilde{S}}I - Q_k^T\tilde{S}\right)Q_k^T$, then
\begin{align*}
	\Lambda(\delta R_k(\hat{x}_k-\hat{\mu}_k)R_k) &= (S_{k+1}U_{k+1}^T\delta R_k(\hat{x}_k-\hat{\mu}_k)U_kQ_kV_k^TV_{k+1} - V_{k+1}^TV_kQ_k^TU_k^T(\hat{x}_k-\hat{\mu}_k)^T\delta R_k^TU_{k+1}S_{k+1})^\vee \\
	&= (S_{k+1}U_{k+1}^T\delta R_kU_k(U_k^T(x_k-\mu_k))^\wedge Q_k\tilde{V}^T - \tilde{V}Q_k^T((U_k^T(x_k-\mu_k))^\wedge)^TU_k^T\delta R_k^TU_{k+1}S_{k+1})^\vee \\
	&= (S_{k+1}\tilde{U}(U_k^T(x_k-\mu_k))^\wedge Q_k\tilde{V}^T - \tilde{V}Q_k^T((U_k^T(x_k-\mu_k))^\wedge)^T\tilde{U}^TS_{k+1})^\vee \\
	&= \tilde{V}(\tilde{S}^T(U_k^T(x_k-\mu_k))^\wedge Q_k - Q_k^T((U_k^T(x_k-\mu_k))^\wedge)^T\tilde{S})^\vee \\
	&= \tilde{V}(\tilde{S}^TQ_k(Q_k^TU_k^T(x_k-\mu_k))^\wedge - ((Q_k^TU_k^T(x_k-\mu_k))^\wedge)^TQ_k^T\tilde{S})^\vee \\
	&= \left(\tr{Q_k^T\tilde{S}}I - Q_k^T\tilde{S}\right)Q_k^TU_k^T(x_k-\mu_k) \\
	&= \tilde{V}\Gamma_QU_k^T(x_k-\mu_k).
\end{align*}

\noindent Therefore, the first term on the right hand side is
\begin{align*}
	\expect{x_k\Lambda(\delta R_kR_k)^T} = \mu_k\expect{\tilde{\nu}}^T\tilde{V}^T + P_k\expect{\nu_{R_k}\tilde{\nu}^T}\tilde{V}^T.
\end{align*}

\noindent The second term on the right hand side is
\begin{align*}
	\expect{x_k\Lambda(\delta R_k(\hat{x}_k-\hat{\mu}_k)R_k)^T} &= \expect{x_k(x_k-\mu_k)^TU_k\Gamma_Q^T}\tilde{V}^T \\
	&= \expect{\left( \Sigma_{c_k} + \mu_k\nu_{R_k}^TP_k^T + P_k\nu_{R_k}\nu_{R_k}^TP_k^T \right)U_k\Gamma_Q^T}\tilde{V}^T \\
	&= \Sigma_{c_k}U_k\expect{\Gamma_Q}^T\tilde{V}^T + \mu_k\expect{\nu_{R_k}^TP_k^TU_k\Gamma_Q^T}\tilde{V}^T + P_k\expect{\nu_{R_k}\nu_{R_k}^TP_k^TU_k\Gamma_Q^T}\tilde{V}^T.
\end{align*}

\noindent Let $\tilde{\tilde{\nu}} = (\tilde{\tilde{S}}^TQ_k - Q_k^T\tilde{\tilde{S}})^\vee$, then the third term on the right hand side is
\begin{align*}
	\expect{x_k\Lambda(\delta R_k((H_u\Delta W_u)^\wedge)^2 R_k)^T} &= h\expect{x_k\Lambda(\delta R_k(G_u-\tr{G_u}I)R_k)^T} \\
	&= h\expect{x_k\Lambda(\delta R_kG_uR_k)^T} - \tr{G_u}h\expect{x_k\Lambda(\delta R_kR_k)^T} \\
	&= h\left(\mu_k\expect{\tilde{\tilde{\nu}}}^T + P_k\expect{\nu_{R_k}\tilde{\tilde{\nu}}^T}\right)\tilde{V}^T - \tr{G_u}h\left( \mu_k\expect{\tilde{\nu}}^T + P_k\expect{\nu_{R_k}\tilde{\nu}^T} \right)\tilde{V}^T.
\end{align*}

\noindent $\Gamma_Q$ can be simplified as
\begin{align*}
	(\Gamma_Q)_{11} &= \tilde{S}_{33}Q_{22} + \tilde{S}_{22}Q_{33} - \tilde{S}_{32}Q_{23} - \tilde{S}_{23}Q_{32} \\
	(\Gamma_Q)_{12} &= \tilde{S}_{32}Q_{13} + \tilde{S}_{13}Q_{32} - \tilde{S}_{33}Q_{12} - \tilde{S}_{12}Q_{33} \\
	(\Gamma_Q)_{13} &= \tilde{S}_{23}Q_{12} + \tilde{S}_{12}Q_{23} - \tilde{S}_{22}Q_{13} - \tilde{S}_{13}Q_{22} \\
	(\Gamma_Q)_{21} &= \tilde{S}_{31}Q_{23} + \tilde{S}_{23}Q_{31} - \tilde{S}_{33}Q_{21} - \tilde{S}_{21}Q_{33} \\
	(\Gamma_Q)_{22} &= \tilde{S}_{33}Q_{11} + \tilde{S}_{11}Q_{33} - \tilde{S}_{31}Q_{13} - \tilde{S}_{13}Q_{31} \\
	(\Gamma_Q)_{23} &= \tilde{S}_{21}Q_{13} + \tilde{S}_{13}Q_{21} - \tilde{S}_{23}Q_{11} - \tilde{S}_{11}Q_{23} \\
	(\Gamma_Q)_{31} &= \tilde{S}_{32}Q_{21} + \tilde{S}_{21}Q_{32} - \tilde{S}_{31}Q_{22} - \tilde{S}_{22}Q_{31} \\
	(\Gamma_Q)_{32} &= \tilde{S}_{31}Q_{12} + \tilde{S}_{12}Q_{31} - \tilde{S}_{32}Q_{11} - \tilde{S}_{11}Q_{32} \\
	(\Gamma_Q)_{33} &= \tilde{S}_{22}Q_{11} + \tilde{S}_{11}Q_{22} - \tilde{S}_{21}Q_{12} - \tilde{S}_{12}Q_{21}.
\end{align*}

\subsection{Calculating $\expect{\nu_{R_{k+1}}\nu_{R_{k+1}}^T}$}

\begin{align*}
	\expect{\nu_{R_{k+1}}\nu_{R_{k+1}}^T} &= \expect{\sum_{i=1}^\infty \Lambda\left( \delta R_k \frac{(h(\hat{x}_k-\hat{\mu}_k)+(H_u\Delta W_u)^\wedge)^i}{i!} R_k \right) \cdot \sum_{i=1}^\infty \Lambda\left( \delta R_k \frac{(h(\hat{x}_k-\hat{\mu}_k)+(H_u\Delta W_u)^\wedge)^i}{i!} R_k \right)^T } \\
	&= \expect{\Lambda(\delta R_kR_k)\Lambda(\delta R_kR_k)^T} + h\expect{\Lambda(\delta R_kR_k)\Lambda(\delta R_k(\hat{x}_k-\hat{\mu}_k) R_k)^T} \\
	&\qquad + h\expect{\Lambda(\delta R_k(\hat{x}_k-\hat{\mu}_k) R_k)\Lambda(\delta R_kR_k)^T} + \frac{1}{2}\expect{\Lambda(\delta R_kR_k)\Lambda(\delta R_k((H_u\Delta W_u)^\wedge)^2R_k)^T} \\
	&\qquad + \frac{1}{2}\expect{\Lambda(\delta R_k((H_u\Delta W_u)^\wedge)^2R_k)\Lambda(\delta R_kR_k)^T} + \expect{\Lambda(\delta R_k(H_u\Delta W_u)^\wedge R_k)\Lambda(\delta R_k(H_u\Delta W_u)^\wedge R_k)^T}.
\end{align*}

\noindent The first term on the right hand side is
\begin{align*}
	\expect{\Lambda(\delta R_kR_k)\Lambda(\delta R_kR_k)^T} = \tilde{V}\expect{\tilde{\nu}\tilde{\nu}^T}\tilde{V}^T.
\end{align*}

\noindent The second, third term on the right hand side is
\begin{align*}
	\expect{\Lambda(\delta R_kR_k)\Lambda(\delta R_k(\hat{x}_k-\hat{\mu}_k)R_k)^T} &= \tilde{V}\expect{\tilde{\nu}(x_k-\mu_k)^TU_k\Gamma_Q^T}\tilde{V}^T \\
	&= \tilde{V}\expect{\tilde{\nu}\nu_{R_k}^TP_k^TU_k\Gamma_Q^T}\tilde{V}^T.
\end{align*}

\noindent The fourth, fifth term on the right hand side is
\begin{align*}
	\expect{\Lambda(\delta R_kR_k)\Lambda(\delta R_k((H_u\Delta W_u)^\wedge)^2R_k)^T} &= h\expect{\Lambda(\delta R_kR_k)\Lambda(\delta R_k(G_u-\tr{G_u}I)R_k)^T} \\
	&= h\tilde{V}\expect{\tilde{\nu}\tilde{\tilde{\nu}}^T}\tilde{V}^T - \tr{G_u}h\tilde{V}\expect{\tilde{\nu}\tilde{\nu}^T}\tilde{V}^T.
\end{align*}

\noindent The sixth term on the right hand side is
\begin{align*}
	\expect{\Lambda(\delta R_k(H_u\Delta W_u)^\wedge R_k)\Lambda(\delta R_k(H_u\Delta W_u)^\wedge R_k)^T} &= \tilde{V}\expect{\Gamma_QU_k^T(H_u\Delta W_u)^\wedge((H_u\Delta W_u)^\wedge)^TU_k\Gamma_Q^T}\tilde{V}^T \\
	&= \tilde{V}\expect{\Gamma_QU_k^TG_uU_k\Gamma_Q^T}\tilde{V}^T.
\end{align*}

\end{document}

